wip verification

src/verification/Contracts.v
@@ -6,7 +6,10 @@ From Coq Require Import
 From Katamaran Require Import
      Notations
      Specification
-     Assertions.
+     Assertions
+     Bitvector
+     MicroSail.SymbolicExecutor
+     MicroSail.Soundness.
 
 Require Import
   Machine
@@ -16,7 +19,7 @@ Set Implicit Arguments.
 Import ctx.resolution.
 Import ctx.notations.
 Import env.notations.
-(* Import bv.notations. *)
+Import bv.notations.
 Import ListNotations.
 Open Scope string_scope.
 Open Scope ctx_scope.
@@ -34,6 +37,9 @@ Module Import MSP430Specification <: Specification MSP430Base MSP430Signature MS
 
   Definition SepContractFunX {Δ τ} (f : FunX Δ τ) : Type :=
     SepContract Δ τ.
+
+  Definition SepLemma {Δ} (f : Lem Δ) : Type :=
+    Lemma Δ.
 
   Section ContractDefKit.
     (* Local Notation "x + y" := (term_binop bop.plus x y). *)
@@ -54,10 +60,22 @@ Module Import MSP430Specification <: Specification MSP430Base MSP430Signature MS
                     | WORD_INSTRUCTION => w
                     end)).
 
-    Local Notation asn_access_allowed addr am pc MPUIPC0 MPUIPSEGB1 MPUIPSEGB2:=
-      (asn.formula (formula_user access_allowed
-                      [addr; term_enum Eaccess_mode am; term_var pc;
-                       term_var MPUIPC0; term_var MPUIPSEGB1; term_var MPUIPSEGB2])).
+    Local Notation asn_ipe_ctl x := (asn.chunk (chunk_user ipe_ctl [term_var x])).
+    Local Notation asn_ipe_ctl_record x := (asn.chunk (chunk_user ipe_ctl [x])).
+
+    Local Notation asn_accessible_addresses ctl :=
+      (asn.chunk (chunk_user accessible_addresses [term_var ctl])).
+
+    Local Notation asn_mpu_pwd_correct ctl := (asn.formula (formula_user mpu_pwd_correct_p [term_var ctl])).
+    Local Notation asn_mpu_pwd_incorrect ctl := (asn.formula (formula_user mpu_pwd_incorrect_p [term_var ctl])).
+    Local Notation asn_ipe_enabled ctl := (asn.formula (formula_user ipe_enabled_p [term_var ctl])).
+    Local Notation asn_ipe_locked ctl := (asn.formula (formula_user ipe_locked_p [term_var ctl])).
+    Local Notation asn_ipe_unlocked ctl := (asn.formula (formula_user ipe_unlocked_p [term_var ctl])).
+
+    Local Notation asn_access_allowed ctl am pc addr :=
+      (asn.formula
+         (formula_user access_allowed_p
+            [term_var ctl; term_enum Eaccess_mode am; term_var pc; addr])).
 
     (* Foreign function contracts *)
 
@@ -68,7 +86,7 @@ Module Import MSP430Specification <: Specification MSP430Base MSP430Signature MS
         sep_contract_localstore      := [term_var "_"];
         sep_contract_precondition    := ⊤;
         sep_contract_result          := "v";
-        sep_contract_postcondition   := ∃ "w", term_var "v" = term_var "w";
+        sep_contract_postcondition   := ⊤;
       |}.
 
     Definition sep_contract_read_ram :
@@ -90,43 +108,170 @@ Module Import MSP430Specification <: Specification MSP430Base MSP430Signature MS
 
         sep_contract_localstore      := [term_var "addr"; term_var "v"];
         sep_contract_precondition    := term_var "addr" m↦ term_var "w";
-        sep_contract_result          := "_";
-        sep_contract_postcondition   := term_var "addr" m↦ term_var "v";
+        sep_contract_result          := "u";
+        sep_contract_postcondition   :=
+          term_var "addr" m↦ term_var "v"
+          ∗ term_var "u" = term_val ty.unit tt;
       |}.
 
     (* μSail function contracts *)
+
+    Definition sep_contract_check_ipe_access :
+      SepContractFun check_ipe_access :=
+      {|
+        sep_contract_logic_variables :=
+          [ "addr"    :: ty.Address
+          ; "m"       :: ty.enum Eaccess_mode
+          ; "ipe_ctl" :: ty.record Ripe_ctl
+          ; "pc"      :: ty.wordBits          ];
+
+        sep_contract_localstore := [term_var "addr"; term_var "m"];
+
+        sep_contract_precondition :=
+            PC_reg ↦ term_var "pc"
+          ∗ asn_ipe_ctl "ipe_ctl"
+          ∗ asn_access_allowed "ipe_ctl" R "pc" (term_var "addr");
+
+        sep_contract_result        := "v";
+        sep_contract_postcondition := ⊤ (* term_var "v" = term_val ty.bool true *);
+      |}.
 
     Definition sep_contract_read_mem_aux :
       SepContractFun read_mem_aux :=
       {|
         sep_contract_logic_variables :=
           ["bw" :: ty.enum Ebw; "addr" :: ty.Address; "m" :: ty.enum Eaccess_mode;
-           "MPUCTL0" :: ty.wordBits; "MPUIPSEGB1" :: ty.wordBits; "MPUIPSEGB2" :: ty.wordBits;
-           "pc" :: ty.wordBits; "vl" :: ty.byteBits; "vh" :: ty.byteBits];
+           "ipe_ctl" :: ty.record Ripe_ctl; "pc" :: ty.wordBits;
+           "vl" :: ty.byteBits; "vh" :: ty.byteBits];
 
         sep_contract_localstore := [term_var "bw"; term_var "addr"; term_var "m"];
 
         sep_contract_precondition :=
+          term_var "m" = term_enum Eaccess_mode R ∗ (* XXX *)
             term_var "addr" m↦ term_var "vl"
           ∗ PC_reg ↦ term_var "pc"
-          ∗ MPUCTL0_reg ↦ term_var "MPUCTL0"
-          ∗ MPUIPSEGB1_reg ↦ term_var "MPUIPSEGB1"
-          ∗ MPUIPSEGB2_reg ↦ term_var "MPUIPSEGB2"
-          ∗ asn_access_allowed (term_var "addr") R "pc" "MPUCTL0" "MPUIPSEGB1" "MPUIPSEGB2"
+          ∗ asn_ipe_ctl "ipe_ctl"
+          ∗ asn_access_allowed "ipe_ctl" R "pc" (term_var "addr")
           ∗ match_bw (term_var "bw")
               ⊤
               (inc "addr" m↦ term_var "vh"
-               ∗ asn_access_allowed (inc "addr") R "pc" "MPUCTL0" "MPUIPSEGB1" "MPUIPSEGB2");
+               ∗ asn_access_allowed "ipe_ctl" R "pc" (inc "addr"));
 
         sep_contract_result          := "w";
-        sep_contract_postcondition   :=
-            term_var "addr" m↦ term_var "vl"
-          ∗ match_bw (term_var "bw")
-              (term_var "w" = term_union Uwordbyte Kbyte (term_var "vl"))
-              (inc "addr" m↦ term_var "vh"
-               ∗ term_var "w" = term_union Uwordbyte Kword (term_var "vh" ++ term_var "vl"));
+        sep_contract_postcondition   := ⊤;
+          (*   term_var "addr" m↦ term_var "vl" *)
+          (* ∗ PC_reg ↦ term_var "pc" *)
+          (* ∗ asn_ipe_ctl "ipe_ctl" *)
+          (* ∗ match_bw (term_var "bw") *)
+          (*     (term_var "w" = term_union Uwordbyte Kbyte (term_var "vl")) *)
+          (*     (inc "addr" m↦ term_var "vh" *)
+          (*      ∗ term_var "w" = term_union Uwordbyte Kword (term_var "vh" ++ term_var "vl")); *)
       |}.
 
+    Definition sep_contract_execute :
+      SepContractFun execute :=
+      {|
+        sep_contract_logic_variables :=
+          [ "ipe_ctl" :: ty.record Ripe_ctl; "pc" :: ty.wordBits
+          ; "instr" :: ty.union Uast ];
+
+        sep_contract_localstore := [term_var "instr"];
+
+        sep_contract_precondition :=
+            PC_reg ↦ term_var "pc"
+          ∗ asn_ipe_ctl "ipe_ctl"
+          ∗ asn_accessible_addresses "ipe_ctl";
+
+        sep_contract_result          := "u";
+        sep_contract_postcondition   :=
+            term_var "u" = term_val ty.unit tt
+          ∗ asn_accessible_addresses "ipe_ctl"
+          ∗ PC_reg ↦ term_var "pc"
+          ∗ (* IPE control registers can change if the password is correct
+               and they are not locked TODO and they are not protected by IPE? *)
+            (asn_mpu_pwd_correct "ipe_ctl" ∗ asn_ipe_unlocked "ipe_ctl"
+             ∗ ∃ "new_ctl", asn_ipe_ctl "new_ctl"
+             ∨ (* otherwise they must stay the same *)
+               asn_ipe_ctl "ipe_ctl");
+      |}.
+
+    (* lemmas *)
+
+    Definition lemma_open_ipe_ctl : SepLemma open_ipe_ctl :=
+      {|
+        lemma_logic_variables := ["ipe_ctl" :: ty.record Ripe_ctl];
+        lemma_patterns        := env.nil;
+        lemma_precondition    := asn_ipe_ctl "ipe_ctl";
+        lemma_postcondition   :=
+          ∃ "mpuctl0", ∃ "ipectl", ∃ "segb1", ∃ "segb2",
+          ( MPUCTL0_reg ↦ term_var "mpuctl0"
+          ∗ MPUIPC0_reg ↦ term_var "ipectl"
+          ∗ MPUIPSEGB1_reg ↦ term_var "segb1"
+          ∗ MPUIPSEGB2_reg ↦ term_var "segb2"
+          ∗ term_var "ipe_ctl" =
+              term_record Ripe_ctl
+                [env]
+                .["mpu_pwd_correct" ∷ ty.bool ↦
+                    term_binop (bop.relop bop.eq)
+                      (term_unop (uop.vector_subrange 8 8) (term_var "mpuctl0"))
+                      (term_val (ty.bvec 8) [bv 0x96])]
+                .["ipe_enabled"     ∷ ty.bool ↦
+                    term_binop (bop.relop bop.eq)
+                      (term_unop (uop.vector_subrange 6 1) (term_var "ipectl"))
+                      (term_val (ty.bvec 1) [bv 1])]
+                .["ipe_locked"      ∷ ty.bool ↦
+                    term_binop (bop.relop bop.eq)
+                      (term_unop (uop.vector_subrange 7 1) (term_var "ipectl"))
+                      (term_val (ty.bvec 1) [bv 1])]
+                .["ipe_low_bound"   ∷ ty.int  ↦
+                    term_binop bop.times
+                      (term_unop uop.unsigned (term_var "segb1"))
+                      (term_val ty.int 16)]
+                .["ipe_high_bound"  ∷ ty.int  ↦
+                    term_binop bop.times
+                      (term_unop uop.unsigned (term_var "segb2"))
+                      (term_val ty.int 16)]
+          );
+      |}.
+
+    Definition lemma_close_ipe_ctl : SepLemma open_ipe_ctl :=
+      {|
+        lemma_logic_variables := [ "mpuctl0" :: ty.wordBits
+                                 ; "ipectl"  :: ty.wordBits
+                                 ; "segb1"   :: ty.wordBits
+                                 ; "segb2"   :: ty.wordBits ];
+        lemma_patterns        := env.nil;
+        lemma_precondition    :=
+            MPUCTL0_reg    ↦ term_var "mpuctl0"
+          ∗ MPUIPC0_reg    ↦ term_var "ipectl"
+          ∗ MPUIPSEGB1_reg ↦ term_var "segb1"
+          ∗ MPUIPSEGB2_reg ↦ term_var "segb2";
+
+        lemma_postcondition   :=
+          asn_ipe_ctl_record
+            (term_record Ripe_ctl
+               [env]
+             .["mpu_pwd_correct" ∷ ty.bool ↦
+                 term_binop (bop.relop bop.eq)
+                 (term_unop (uop.vector_subrange 8 8) (term_var "mpuctl0"))
+                 (term_val (ty.bvec 8) [bv 0x96])]
+             .["ipe_enabled"     ∷ ty.bool ↦
+                 term_binop (bop.relop bop.eq)
+                 (term_unop (uop.vector_subrange 6 1) (term_var "ipectl"))
+                 (term_val (ty.bvec 1) [bv 1])]
+             .["ipe_locked"      ∷ ty.bool ↦
+                 term_binop (bop.relop bop.eq)
+                 (term_unop (uop.vector_subrange 7 1) (term_var "ipectl"))
+                 (term_val (ty.bvec 1) [bv 1])]
+             .["ipe_low_bound"   ∷ ty.int  ↦
+                 term_binop bop.times
+                 (term_unop uop.unsigned (term_var "segb1"))
+                 (term_val ty.int 16)]
+             .["ipe_high_bound"  ∷ ty.int  ↦
+                 term_binop bop.times
+                 (term_unop uop.unsigned (term_var "segb2"))
+                 (term_val ty.int 16)]);
+      |}.
 
     (* The following maps μSail function names to their contracts. *)
     Definition CEnv : SepContractEnv :=
@@ -149,6 +294,48 @@ Module Import MSP430Specification <: Specification MSP430Base MSP430Signature MS
     Definition LEnv : LemmaEnv :=
       fun Δ l =>
         match l with
+        | open_ipe_ctl => lemma_open_ipe_ctl
+        | close_ipe_ctl => lemma_close_ipe_ctl
         end.
   End ContractDefKit.
 End MSP430Specification.
+
+(*** VERIFICATION ***)
+
+Import MSP430Specification.
+Import Erasure.notations.
+
+Module MSP430Executor :=
+  MakeExecutor MSP430Base MSP430Signature MSP430Program MSP430Specification.
+
+Import MSP430Executor.
+Import MSP430Executor.Symbolic.
+
+Ltac symbolic_simpl :=
+  apply validcontract_with_erasure_sound;
+  compute;
+  constructor;
+  cbn.
+
+Lemma valid_contract_check_ipe_access : Symbolic.ValidContract sep_contract_check_ipe_access fun_check_ipe_access.
+Proof.
+  apply validcontract_with_erasure_sound.
+  compute.
+
+  symbolic_simpl.
+  (* unfold access_allowed_inst.
+  unfold ipe_enabled.
+   *)
+  (* intros. *)
+
+Lemma valid_contract_read_mem_aux : Symbolic.ValidContract sep_contract_read_mem_aux fun_read_mem_aux.
+Proof.
+  symbolic_simpl.
+  intros bw v _ ctl w _ _ Haccess.
+  split.
+  - intro.
+    unfold access_allowed_inst.
+    .
+
+Lemma valid_contract_execute : Symbolic.ValidContractReflect sep_contract_execute fun_execute.
+Proof. reflexivity. Qed.
