src/verification/Sig.v
@@ -24,10 +24,17 @@ Open Scope string_scope.
 Open Scope Z_scope.
 
 Inductive PurePredicate : Set :=
-| access_allowed.
+| mpu_pwd_correct_p
+| mpu_pwd_incorrect_p
+| ipe_enabled_p
+| ipe_locked_p
+| ipe_unlocked_p
+| access_allowed_p.
 
 Inductive Predicate :=
-| ptstomem.
+| ptstomem
+| ipe_ctl
+| accessible_addresses.
 
 Section TransparentObligations.
   Local Set Transparent Obligations.
@@ -46,57 +53,53 @@ Module Export MSP430Signature <: Signature MSP430Base.
     Local Definition get_bit {n} (v : bv n) (i : nat) {p : IsTrue (Nat.leb (i + 1) n)}: bool :=
       bv.msb (@bv.vector_subrange n i 1 p v).
 
-    (* Definition ipe_enabled (MPUIPC0 : Val (ty.wordBits)) : Prop :=
-      get_bit MPUIPC0 6 = true.
-
-    Definition in_ipe_segment
-      (addr          : Val ty.Address)
-      (MPUIPSEGB1    : Val ty.wordBits)
-      (MPUIPSEGB2    : Val ty.wordBits)
-      (low_bound_off : Z)
-      : Prop
-    :=
-      let addr := bv.unsigned addr in
-      let low  := (bv.unsigned MPUIPSEGB1 * 16)%Z + low_bound_off in
-      let high := (bv.unsigned MPUIPSEGB2 * 16)%Z in
-      Z.le low addr /\ Z.lt addr high. *)
+    Definition mpu_pwd_correct_inst (ctl : Val (ty.record Ripe_ctl)) := mpu_pwd_correct ctl = true.
+    Definition mpu_pwd_incorrect_inst (ctl : Val (ty.record Ripe_ctl)) := mpu_pwd_correct ctl = false.
+    Definition ipe_enabled_inst (ctl : Val (ty.record Ripe_ctl)) := ipe_enabled ctl = true.
+    Definition ipe_locked_inst (ctl : Val (ty.record Ripe_ctl)) := ipe_locked ctl = true.
+    Definition ipe_unlocked_inst (ctl : Val (ty.record Ripe_ctl)) := ipe_locked ctl = false.
 
     Definition access_allowed_inst
-      (addr       : Val ty.Address)
-      (am         : Val (ty.enum Eaccess_mode))
-      (pc         : Val ty.wordBits)
-      (MPUIPC0    : Val ty.wordBits)
-      (MPUIPSEGB1 : Val ty.wordBits)
-      (MPUIPSEGB2 : Val ty.wordBits)
+      (ctl  : Val (ty.record Ripe_ctl))
+      (am   : Val (ty.enum Eaccess_mode))
+      (pc   : Val ty.wordBits)
+      (addr : Val ty.Address)
       : Prop
     :=
       let addr := bv.unsigned addr in
       let pc   := bv.unsigned pc in
-      let low  := (bv.unsigned MPUIPSEGB1 * 16)%Z in
-      let high := (bv.unsigned MPUIPSEGB2 * 16)%Z in
+      let low  := ipe_low_bound ctl in
+      let high := ipe_high_bound ctl in
 
-    (* IPE disabled *)
-    get_bit MPUIPC0 6 = false
-    (* address not in IPE segment *)
-    \/ (Z.lt addr low \/ Z.le high addr)
-    \/ ((* PC in IPE segment except first 8 bytes *)
-        Z.le (low + 8) pc /\ Z.lt pc high
-        (* not execute access in IVT or RV (9.4.1) *)
-        /\ ((Z.lt addr 0xFF80 \/ Z.le 0xFFFF addr)
-            \/ am <> X)).
+      (* IPE disabled *)
+      ipe_enabled ctl = false
+      (* address not in IPE segment *)
+      \/ (Z.lt addr low \/ Z.le high addr)
+      \/ ((* PC in IPE segment except first 8 bytes *)
+          Z.le (low + 8) pc /\ Z.lt pc high
+          (* not execute access in IVT or RV (9.4.1) *)
+          /\ ((Z.lt addr 0xFF80 \/ Z.le 0xFFFF addr)
+              \/ am <> X)).
 
     Definition 𝑷 := PurePredicate.
 
     (* Maps each pure predicate to a list of arguments with their types. *)
     Definition 𝑷_Ty (p : 𝑷) : Ctx Ty :=
       match p with
-      | access_allowed => [ty.Address; ty.enum Eaccess_mode; ty.wordBits; ty.wordBits; ty.wordBits; ty.wordBits]
+      | mpu_pwd_correct_p | mpu_pwd_incorrect_p | ipe_enabled_p
+      | ipe_locked_p | ipe_unlocked_p => [ty.record Ripe_ctl]
+      | access_allowed_p => [ty.record Ripe_ctl; ty.enum Eaccess_mode; ty.wordBits; ty.Address]
       end.
 
     (* Interprets a pure predicate name as a Coq proposition. *)
     Definition 𝑷_inst (p : 𝑷) : env.abstract Val (𝑷_Ty p) Prop :=
       match p with
-      | access_allowed => access_allowed_inst
+      | mpu_pwd_correct_p => mpu_pwd_correct_inst
+      | mpu_pwd_incorrect_p => mpu_pwd_incorrect_inst
+      | ipe_enabled_p => ipe_enabled_inst
+      | ipe_locked_p => ipe_locked_inst
+      | ipe_unlocked_p => ipe_unlocked_inst
+      | access_allowed_p => access_allowed_inst
       end.
 
     Instance 𝑷_eq_dec : EqDec 𝑷 := PurePredicate_eqdec.
@@ -107,6 +110,8 @@ Module Export MSP430Signature <: Signature MSP430Base.
     Definition 𝑯_Ty (p : 𝑯) : Ctx Ty :=
       match p with
       | ptstomem => [ty.Address; ty.byteBits]
+      | ipe_ctl => [ty.record Ripe_ctl]
+      | accessible_addresses => [ty.record Ripe_ctl]
       end.
 
     (* 𝑯_is_dup specifies which predicates are duplicable. A spatial predicate can
@@ -119,23 +124,41 @@ Module Export MSP430Signature <: Signature MSP430Base.
 
     Instance 𝑯_eq_dec : EqDec 𝑯 := Predicate_eqdec.
 
+    Local Arguments Some {_} &.
+
     (* 𝑯_precise specifies which predicates are precise and gives information
      about the input and output parameters of a predicate. *)
-    Definition 𝑯_precise (p : 𝑯) : option (Precise 𝑯_Ty p) := None.
+    Definition 𝑯_precise (p : 𝑯) : option (Precise 𝑯_Ty p) :=
+      match p with
+      | ipe_ctl => Some (MkPrecise ε [ty.record Ripe_ctl] eq_refl)
+      | _ => None
+      end.
 
   End PredicateKit.
 
   Include PredicateMixin MSP430Base.
   Include WorldsMixin MSP430Base.
 
-  (* In the MinCapsSolverKit we provide simplification procedures for the pure
+  (* In the MSP430SolverKit we provide simplification procedures for the pure
      predicates and prove that these simplifiers are sound. *)
   Section MSP430SolverKit.
-    Definition solver : Solver := fun _ _ => None.
+    Import Entailment.
+
+    Definition solve_user : SolverUserOnly :=
+      fun Σ p ts => Some [formula_user p ts]%ctx.
+
+    Definition solver : Solver := solveruseronly_to_solver solve_user.
+
+    Lemma solve_user_spec : SolverUserOnlySpec solve_user.
+    Proof.
+      intros Σ p ts.
+      destruct p; cbv in ts; env.destroy ts; reflexivity.
+    Qed.
 
     Lemma solver_spec : SolverSpec solver.
     Proof.
-    Admitted.
+      apply solveruseronly_to_solver_spec, solve_user_spec.
+    Qed.
   End MSP430SolverKit.
 
   Include SignatureMixin MSP430Base.
