src/verification/Base.v
@@ -268,7 +268,14 @@ Inductive Unions : Set :=
   | Uwordbyte 
   | Uast      .
 
-Inductive Records : Set :=.
+Record IPEctl : Set := mkIPEctl
+  { mpu_pwd_correct : bool
+  ; ipe_enabled     : bool
+  ; ipe_locked      : bool
+  ; ipe_low_bound   : Z
+  ; ipe_high_bound  : Z }.
+
+Inductive Records : Set := Ripe_ctl.
 
 Section TransparentObligations.
   Local Set Transparent Obligations.
@@ -291,6 +298,7 @@ Section TransparentObligations.
   Derive NoConfusion for Unions.
   Derive NoConfusion for Records.
   Derive NoConfusion for RegName.
+  Derive NoConfusion for IPEctl.
 End TransparentObligations.
 
 Derive EqDec for exception.
@@ -311,6 +319,7 @@ Derive EqDec for Enums.
 Derive EqDec for Unions.
 Derive EqDec for Records.
 Derive EqDec for RegName.
+Derive EqDec for IPEctl.
 
 Section Finite.
   Import stdpp.finite.
@@ -512,6 +521,7 @@ Module Export MSP430Base <: Base.
   
   Definition record_denote (r : Records) : Set :=
     match r with
+    | Ripe_ctl => IPEctl
     end.
   
   #[export] Instance typedenotekit : TypeDenoteKit typedeclkit :=
@@ -621,18 +631,27 @@ Module Export MSP430Base <: Base.
                               | DOESNOTUNDERSTAND ж1            => existT Kdoesnotunderstand ж1
                               end
     end.
-  
+
   Definition record_field_type (R : recordi) : NCtx string Ty :=
     match R with
+    | Ripe_ctl => [ "mpu_pwd_correct" :: ty.bool
+                  ; "ipe_enabled"     :: ty.bool
+                  ; "ipe_locked"      :: ty.bool
+                  ; "ipe_low_bound"   :: ty.int
+                  ; "ipe_high_bound"  :: ty.int ]
     end.
-  
-  Definition record_fold (R : recordi) : NamedEnv Val (record_field_type R) -> recordt R :=
-    match R with
-    end%exp.
-  
-  Definition record_unfold (R : recordi) : recordt R -> NamedEnv Val (record_field_type R) :=
-    match R with
-    end%env.
+
+   Equations record_fold (R : recordi) : NamedEnv Val (record_field_type R) -> recordt R :=
+   | Ripe_ctl , [pwd; en; lk; lo; hi]%env := mkIPEctl pwd en lk lo hi.
+
+   Equations record_unfold (R : recordi) : recordt R -> NamedEnv Val (record_field_type R) :=
+   | Ripe_ctl , r =>
+       env.nil
+         ► ("mpu_pwd_correct" :: ty.bool ↦ mpu_pwd_correct r)
+         ► ("ipe_enabled"     :: ty.bool ↦ ipe_enabled     r)
+         ► ("ipe_locked"      :: ty.bool ↦ ipe_locked      r)
+         ► ("ipe_low_bound"   :: ty.int  ↦ ipe_low_bound   r)
+         ► ("ipe_high_bound"  :: ty.int  ↦ ipe_high_bound  r).
   
   #[export,refine] Instance typedefkit : TypeDefKit typedenotekit :=
     {| unionk           := union_constructor;
@@ -769,13 +788,11 @@ Module Export MSP430Base <: Base.
                 ]
       |}.
   End RegDeclKit.
-  
+
   Section MemoryModel.
-    (*TODO*)
-    Definition Memory :=
-      Z -> Z.
+    Definition Memory := Address -> byteBits.
   End MemoryModel.
-  
+
   Include BaseMixin.
 End MSP430Base.
 
